{
 "cells": [
  {
   "cell_type": "markdown",
   "id": "21930e6d",
   "metadata": {},
   "source": [
    "(Lecture2)=\n",
    "\n",
    "# Lecture2 - responses to inputs & complexify\n",
    "\n",
    "## Response to exponential input\n",
    "Consider an ODE: \n",
    "\\begin{eqnarray}\n",
    "\\frac{dy}{dt}=ay+e^{st},\n",
    "\\end{eqnarray}\n",
    "where a and s are known. We call y(t) the \"exponential response\" and exponential term on right hand side the \"input\" or \"forcing\".\n",
    "\n",
    "Assume initial condition at t =0: $$y=y(0)$$, we now look for particular solution in the form of:\n",
    "$$y_{p}(t) = Ye^{st}$$\n",
    "\n",
    "Plug it into the ODE, we can get\n",
    "$$Yse^{st} = aYe^{st} + e^{st} \\rightarrow Ys=Ya+1 \\rightarrow (s-a)Y=1 \\rightarrow Y=\\frac{1}{s-a}$$\n",
    "\n",
    "The complete solution is\n",
    "$$y(t)=y_{p}(t)+y_{h}(t) = \\frac{e^{st}}{s-a} + Ce^{at}$$\n",
    "\n",
    "To determine C, we use the initial condition\n",
    "$$y(0)=\\frac{1}{s-a}+C \\rightarrow C = y(0) - \\frac{1}{s-a}$$\n",
    "\n",
    "So the solution is\n",
    "$$y(t) = \\frac{e^{st}}{s-a} + [y(0)-\\frac{1}{s-a}]e^{at} = \\frac{e^{st}-e^{at}}{s-a}+y(0)e^{at}$$\n",
    "\n",
    "We also define the very particular solution\n",
    "$$y_{vp}(t) = \\frac{e^{st}-e^{at}}{s-a} \\rightarrow y_{vp}(0) = 0$$\n",
    "\n",
    "Note that we can calculate the very particular solution this way:\n",
    "$$\n",
    "y_{vp} = \\int_{0}^{t}e^{a(t-x)}e^{sx}dx = e^{at}\\int_{0}^{t}e^{(s-a)x}dx = e^{at}\\frac{1}{s-a}e^{(s-a)x}\n",
    " \\verb|\\||^{x=t}_{x=0} \\\n",
    "=\\frac{e^{st}-e^{at}}{s-a}\n",
    "$$\n",
    "````{prf:example}\n",
    ":label: my-example_exp_response1\n",
    "If s=a, then the resonance occurs.\n",
    "What is the solution? How can we get the solution?\n",
    "We can use L'Hospital's rule:\n",
    "$$\n",
    "\\lim_{s\\rightarrow a} \\frac{\\frac{d}{ds}(e^{st}-e^{at})}{\\frac{d}{ds}(s-a)} \n",
    "= \\lim_{s\\rightarrow a} \\frac{te^{st}}{1} = te^{at}\n",
    "$$\n",
    "````\n",
    "## Response to oscillating input\n",
    "\n",
    "Consider an ODE:\n",
    "\\begin{eqnarray}\n",
    "\\frac{dy}{dt}=ay+\\cos (\\omega t), y(0) = y_{0},\n",
    "\\end{eqnarray}\n",
    "\n",
    "We look for particular solution (we already know homogeneours solution, right?) in the form of:\n",
    "$$\n",
    "y_{p}(t) = M\\cos (\\omega t) + N\\sin (\\omega t)\n",
    "$$\n",
    "\n",
    "Plug it into the ODE:\n",
    "$$\n",
    "-\\omega M\\sin (\\omega t) + \\omega N \\cos (\\omega t) = aM\\cos (\\omega t) + aN\\sin (\\omega t) + \\cos (\\omega t)\n",
    "$$\n",
    "\n",
    "Compare the coefficients:\n",
    "$$\n",
    "-aM+\\omega N = 1, -\\omega M - aN = 0\n",
    "$$\n",
    "\n",
    "We can use matrix-vector form (linear algebra) to solve M and N, right?\n",
    "$$\n",
    "\\rightarrow M = \\frac{-a}{\\omega{^2}+a^{2}}, N = \\frac{\\omega}{\\omega{^2}+a^{2}}\n",
    "$$\n",
    "\n",
    "We could also consider the polar form:\n",
    "$$\n",
    "y_{p}(t) = G\\cos (\\omega t - \\alpha) = G(\\cos (\\omega t)\\cos (\\alpha)+\\sin (\\omega t)\\sin (\\alpha))\n",
    "$$\n",
    "\n",
    "So that\n",
    "$$\n",
    "M=G\\cos (\\alpha), N=G\\sin (\\alpha),\n",
    "$$\n",
    "$$\n",
    "M^{2} + N^{2} = G^{2} \\rightarrow G = \\sqrt{M^{2}+N^{2}}\n",
    "$$\n",
    "$$\n",
    "\\frac{G\\sin (\\alpha)}{G\\cos (\\alpha)} = \\frac{N}{M} \\rightarrow \\tan (\\alpha) = \\frac{N}{M}\n",
    "$$\n",
    "\n",
    "And that\n",
    "$$\n",
    "\\frac{dy}{dt}=G(-\\sin (\\omega t-\\alpha))\\omega = aG\\cos (\\omega t-\\alpha) + \\cos (\\omega t)\n",
    "$$\n",
    "$$\n",
    "\\rightarrow -G(\\sin (\\omega t)\\cos (\\alpha) - \\sin (\\alpha)\\cos (\\omega t)) = aG(\\cos (\\omega t)\\cos (\\alpha)+\\sin (\\omega t)\\sin (\\alpha)) + \\cos (\\omega t)\n",
    "$$\n",
    "$$\n",
    "\\rightarrow G(\\sin (\\alpha)\\cos (\\omega t) - \\sin (\\omega t)\\cos (\\alpha) - a\\cos (\\omega t)\\cos (\\alpha)-a\\sin (\\omega t)\\sin (\\alpha)) = \\cos (\\omega t)\n",
    "$$\n",
    "\n",
    "## Formula for calculating very particular solution\n",
    "To this end, I would like to recap the forumla mentioned in previous lecture:\n",
    "$$\n",
    "\\frac{dy}{dt} = ay + q(t),\n",
    "$$\n",
    "where q(t) is the input.\n",
    "\\begin{eqnarray}\n",
    "y_{vp}(t) = \\int_{s=0}^{s=t}e^{a(t-s)}q(s)ds = e^{at}\\int_{s=0}^{s=t}e^{-as}q(s)ds\n",
    "\\end{eqnarray}\n",
    "\n",
    "And the general or complete solution is\t\n",
    "$$\n",
    "y(t) = y(0)e^{at} + e^{at}\\int_{s=0}^{s=t}e^{-as}q(s)ds\n",
    "$$\n",
    "\n",
    "Check \n",
    "$$\n",
    "\\frac{dy_{vp}}{dt} = ay_{vp} + q(t), y_{vp}(0) = 0\n",
    "$$\n",
    "\n",
    "## Response to constant input\n",
    "Assume q(t) is equal to a constant C, then the general or complete solution is:\n",
    "\\begin{eqnarray}\n",
    "y(t) &=& y(0)e^{at} + e^{at}\\int_{s=0}^{s=t}e^{-as}Cds\\\\\n",
    "&=& y(0)e^{at} + Ce^{at}(\\frac{-1}{a})e^{-as}\\verb|||^{s=t}_{s=0} \\\\\n",
    "&=& y(0)e^{at} + Ce^{at}(\\frac{-1}{a})(e^{-at}-1) \\\\\n",
    "&=& y(0)e^{at} + (\\frac{C}{a}e^{at}-\\frac{C}{a}) \\\\\n",
    "&=& y(0)e^{at} + \\frac{C}{a}(e^{at}-1) \\\\\n",
    "&=& y(0)e^{at} - y_{\\infty}e^{at} + y_{\\infty} \\\\\n",
    "&\\rightarrow& y(t) - y_{infty} = e^{at}(y(0)-y_{infty})\n",
    "\\end{eqnarray}\n",
    "- if a>0 and C.0, then y(t) grows or amplieis IC.\n",
    "- if a<0, then y(t) approach = -c/a.\n",
    "\n",
    "## Response to complex exponential input"
   ]
  }
 ],
 "metadata": {
  "jupytext": {
   "text_representation": {
    "extension": ".md",
    "format_name": "myst"
   }
  },
  "kernelspec": {
   "display_name": "Python 3",
   "language": "python",
   "name": "python3"
  },
  "source_map": [
   10
  ]
 },
 "nbformat": 4,
 "nbformat_minor": 5
}